feat: alpha_equiv verify

qcp/ast/annotated_C/alpha_equiv.c
@@ -5,8 +5,9 @@ bool alpha_equiv(term *t1, term *t2)
 /*@ With term1 term2
       Require store_term(t1, term1) *
               store_term(t2, term2)
-      Ensure __return == term_alpha_eqn(term1, term2) && t1 == t1@pre && t2 == t2@pre
-   && store_term(t1, term1) * store_term(t2, term2)
+      Ensure (__return == 1 && term_alpha_eq(term1, term2) || __return == 0 && !term_alpha_eq(term1, term2))
+       && t1 == t1@pre && t2 == t2@pre
+       && store_term(t1, term1) * store_term(t2, term2)
 */
 {
   if (t1 == (void *)0 || t2 == (void *)0) return 0;
@@ -141,6 +142,8 @@ bool alpha_equiv(term *t1, term *t2)
         */
         char *new_var = fresh(t1, t2);
         /*@ 
+            termtypeID(term1) == 3 &&
+            termtypeID(term1) == termtypeID(term2) &&
             store_term(t1, term1) * store_term(t2, term2)
             which implies
             exists y1 z1 qt1 qv1 qterm1 y2 z2 qt2 qv2 qterm2,
@@ -164,6 +167,7 @@ bool alpha_equiv(term *t1, term *t2)
         free_term(new_t1);
         free_term(new_t2);
         free_str(new_var);
+        return result;
       }
     }
   }
