qcp/ast/VC/alpha_equiv_proof_manual.v
@@ -21,94 +21,360 @@ From SimpleC.EE Require Import malloc.
 From SimpleC.EE Require Import sll_tmpl.
 Local Open Scope sac.
 
-Lemma proof_of_alpha_equiv_entail_wit_1_1 : alpha_equiv_entail_wit_1_1.
-Proof. Admitted. 
-
-Lemma proof_of_alpha_equiv_entail_wit_1_2 : alpha_equiv_entail_wit_1_2.
-Proof. Admitted. 
+Lemma proof_of_alpha_equiv_entail_wit_1 : alpha_equiv_entail_wit_1.
+Proof.
+  pre_process.
+  unfold termtypeID in *.
+  destruct term1; lia.
+Qed.
 
 Lemma proof_of_alpha_equiv_return_wit_1_1 : alpha_equiv_return_wit_1_1.
-Proof. 
-    pre_process.
-    unfold list_Z_cmp in H0.
-    destruct (list_Z_eqb str1 str2) eqn:Heq; [ contradiction | ].
-    unfold store_term, term_alpha_eqn, prop_to_z.
-    rewrite H3, H4.
-    Exists y z.
-    entailer!.
-    destruct (term_alpha_eq_dec (TermVar str1) (TermVar str2)) as [Halpha | Hnotalpha].
-    + inversion Halpha.
-      pose proof list_Z_eq2eqb str1 str2 H13.
-      congruence.
-    + reflexivity.
+Proof.
+  pre_process.
+  rewrite <- derivable1_orp_intros1.
+  rewrite H3, H4.
+  unfold store_term.
+  Exists y z.
+  entailer!.
+  intros Hc.
+  inversion Hc.
+  pose proof list_Z_eq2eqb str1 str2 H13.
+  unfold list_Z_cmp in H0.
+  rewrite H14 in H0.
+  congruence.
 Qed.
 
 Lemma proof_of_alpha_equiv_return_wit_1_2 : alpha_equiv_return_wit_1_2.
-Proof. Admitted. 
+Proof.
+  pre_process.
+  rewrite <- derivable1_orp_intros2.
+  rewrite H3, H4.
+  unfold store_term.
+  Exists y z.
+  entailer!.
+  apply AlphaVar.
+  unfold list_Z_cmp in H0.
+  rewrite H in H0.
+  destruct (list_Z_eqb str1 str2) eqn:Heq; [ | congruence].
+  apply (list_Z_eqb2eq str1 str2 Heq).
+Qed.
 
 Lemma proof_of_alpha_equiv_return_wit_2 : alpha_equiv_return_wit_2.
-Proof. Admitted. 
+Proof.
+  pre_process.
+  rewrite <- derivable1_orp_intros1.
+  rewrite H3, H2.
+  unfold store_term.
+  entailer!.
+  intros Hc; inversion Hc.
+  congruence.
+Qed.  
 
 Lemma proof_of_alpha_equiv_return_wit_3_1 : alpha_equiv_return_wit_3_1.
-Proof. Admitted. 
+Proof.
+  pre_process.
+  rewrite <- derivable1_orp_intros1.
+  rewrite H4, H5.
+  unfold store_term.
+  entailer!.
+  intros Hc; inversion Hc.
+  destruct H18; try congruence. 
+Qed.
 
 Lemma proof_of_alpha_equiv_return_wit_3_2 : alpha_equiv_return_wit_3_2.
-Proof. Admitted. 
+Proof.
+  pre_process.
+  rewrite <- derivable1_orp_intros2.
+  rewrite H4, H5.
+  unfold store_term.
+  entailer!.
+  apply AlphaConst; [auto | right; auto].
+Qed.
 
 Lemma proof_of_alpha_equiv_return_wit_4 : alpha_equiv_return_wit_4.
-Proof. Admitted. 
+Proof.
+  pre_process.
+  rewrite <- derivable1_orp_intros2.
+  rewrite H4, H3.
+  unfold store_term.
+  entailer!.
+  apply AlphaConst; [auto | left; auto].
+Qed.
 
 Lemma proof_of_alpha_equiv_return_wit_5_1 : alpha_equiv_return_wit_5_1.
-Proof. Admitted. 
+Proof.
+  pre_process.
+  rewrite <- derivable1_orp_intros2.
+  rewrite H8, H7.
+  unfold store_term; fold store_term.
+  Exists y1 z1 y2 z2.
+  entailer!.
+  apply AlphaApply; try auto.
+Qed.
 
 Lemma proof_of_alpha_equiv_return_wit_5_2 : alpha_equiv_return_wit_5_2.
-Proof. Admitted. 
+Proof.
+  pre_process.
+Qed.
 
 Lemma proof_of_alpha_equiv_return_wit_5_3 : alpha_equiv_return_wit_5_3.
-Proof. Admitted. 
+Proof. 
+  pre_process.
+Qed.
+
+Lemma proof_of_alpha_equiv_return_wit_5_4 : alpha_equiv_return_wit_5_4.
+Proof.
+  pre_process.
+  rewrite <- derivable1_orp_intros1.
+  rewrite H7, H8.
+  unfold store_term; fold store_term.
+  Exists y1 z1 y2 z2.
+  entailer!.
+  contradict H1.
+  inversion H1.
+  auto.
+Qed.
+
+Lemma proof_of_alpha_equiv_return_wit_5_5 : alpha_equiv_return_wit_5_5.
+Proof.
+  pre_process.
+Qed.
+
+Lemma proof_of_alpha_equiv_return_wit_5_6 : alpha_equiv_return_wit_5_6.
+Proof.
+  pre_process.
+  rewrite <- derivable1_orp_intros1.
+  rewrite H4, H5.
+  unfold store_term; fold store_term.
+  Exists y1 z1 y2 z2.
+  entailer!.
+  contradict H1.
+  inversion H1.
+  auto.
+Qed.
 
 Lemma proof_of_alpha_equiv_return_wit_6 : alpha_equiv_return_wit_6.
-Proof. Admitted. 
+Proof.
+  pre_process.
+  rewrite <- derivable1_orp_intros1.
+  rewrite H2, H3.
+  unfold store_term; fold store_term.
+  Exists y1 z1 y2 z2.
+  entailer!.
+  contradict H.
+  inversion H.
+  auto.
+Qed.
 
-Lemma proof_of_alpha_equiv_return_wit_7 : alpha_equiv_return_wit_7.
-Proof. Admitted. 
+Lemma proof_of_alpha_equiv_return_wit_7_1 : alpha_equiv_return_wit_7_1.
+Proof.
+  pre_process.
+  rewrite <- derivable1_orp_intros2.
+  rewrite H6, H7.
+  unfold store_term; fold store_term.
+  Exists y1 z1 y2 z2.
+  entailer!.
+  apply AlphaQuant; [auto | left; split; [ | auto]].
+  unfold list_Z_cmp in H2.
+  destruct (list_Z_eqb qv1 qv2) eqn:Heq; [reflexivity | congruence].
+Qed.
+
+Lemma proof_of_alpha_equiv_return_wit_7_2 : alpha_equiv_return_wit_7_2.
+Proof.
+  pre_process.
+  rewrite <- derivable1_orp_intros1.
+  rewrite H6, H7.
+  unfold store_term; fold store_term.
+  Exists y1 z1 y2 z2.
+  entailer!.
+  contradict H0.
+  inversion H0.
+  destruct H24 as [[Ha Hb] | Hc].
+  + auto.
+  + destruct Hc as [x Hx].
+  Admitted. 
 
 Lemma proof_of_alpha_equiv_return_wit_8_1 : alpha_equiv_return_wit_8_1.
-Proof. Admitted. 
+Proof. 
+    pre_process.
+    rewrite H, H7, H8.
+    rewrite <- derivable1_orp_intros2.
+    unfold store_term; fold store_term.
+    Exists y1 z1 y2 z2.
+    entailer!.
+    apply AlphaQuant.
+    + rewrite H7 in H16; injection H16; intros.
+      rewrite H8 in H17; injection H17; intros.
+      rewrite H29, H32; exact H13.
+    + right; exists str.
+      rewrite <- H7, <- H8.
+      auto.
+Qed.
 
 Lemma proof_of_alpha_equiv_return_wit_8_2 : alpha_equiv_return_wit_8_2.
-Proof. Admitted. 
+Proof.
+  pre_process.
+  rewrite H, H7, H8.
+  rewrite <- derivable1_orp_intros1.
+  unfold store_term; fold store_term.
+  Exists y1 z1 y2 z2.
+  entailer!.
+  contradict H0.
+  inversion H0.
+  destruct H34 as [Ha|Hb].
+  + destruct Ha as [Hc Hd].
+    admit.
+  + destruct Hb as [x Hx]. 
+  
+  Admitted. 
 
-Lemma proof_of_alpha_equiv_return_wit_9 : alpha_equiv_return_wit_9.
-Proof. Admitted. 
+Lemma proof_of_alpha_equiv_return_wit_9_1 : alpha_equiv_return_wit_9_1.
+Proof. 
+  pre_process.
+  rewrite H.
+  rewrite <- derivable1_orp_intros1.
+  pose proof store_term_unfold 0 term2.
+  Admitted. 
 
-Lemma proof_of_alpha_equiv_partial_solve_wit_15_pure : alpha_equiv_partial_solve_wit_15_pure.
-Proof. Admitted. 
+Lemma proof_of_alpha_equiv_return_wit_9_2 : alpha_equiv_return_wit_9_2.
+Proof.
+  pre_process.
+  rewrite H.
+  rewrite <- derivable1_orp_intros1.
+  pose proof store_term_unfold 0 term1.
+  Admitted. 
 
-Lemma proof_of_alpha_equiv_partial_solve_wit_17_pure : alpha_equiv_partial_solve_wit_17_pure.
-Proof. Admitted. 
+Lemma proof_of_alpha_equiv_return_wit_10 : alpha_equiv_return_wit_10.
+Proof.
+  pre_process.
+  rewrite <- derivable1_orp_intros1.
+  Admitted. 
 
-Lemma proof_of_alpha_equiv_partial_solve_wit_21_pure : alpha_equiv_partial_solve_wit_21_pure.
-Proof. Admitted. 
+Lemma proof_of_alpha_equiv_partial_solve_wit_16_pure : alpha_equiv_partial_solve_wit_16_pure.
+Proof. 
+  pre_process.
+  unfold store_string, NULL.
+  Intros n1 n2 n3.
+  entailer!.
+Qed.
+
+Lemma proof_of_alpha_equiv_partial_solve_wit_18_pure : alpha_equiv_partial_solve_wit_18_pure.
+Proof.
+  pre_process.
+  unfold store_string, NULL.
+  Intros n1 n2 n3.
+  entailer!.
+Qed.
+
+Lemma proof_of_alpha_equiv_partial_solve_wit_24_pure : alpha_equiv_partial_solve_wit_24_pure.
+Proof. 
+  pre_process.
+  unfold store_string, NULL.
+  Intros n1 n2 n3.
+  entailer!.
+Qed. 
+
+Lemma proof_of_alpha_equiv_partial_solve_wit_25_pure : alpha_equiv_partial_solve_wit_25_pure.
+Proof. 
+  pre_process.
+  unfold store_string, NULL.
+  Intros n1 n2 n3.
+  entailer!.
+Qed. 
 
 Lemma proof_of_alpha_equiv_which_implies_wit_1 : alpha_equiv_which_implies_wit_1.
-Proof. Admitted. 
+Proof.
+  pre_process.
+  sep_apply store_term_unfold.
+  sep_apply store_term_unfold.
+  unfold NULL.
+  entailer!.
+Qed.
 
 Lemma proof_of_alpha_equiv_which_implies_wit_2 : alpha_equiv_which_implies_wit_2.
-Proof. Admitted. 
+Proof. 
+  pre_process.
+  sep_apply store_term'_Var; unfold NULL.
+  Intros v1 y1.
+  sep_apply store_term'_Var; unfold NULL.
+  Intros v2 y2.
+  Exists y2 y1 v2 v1.
+  entailer!.
+  + auto.
+  + rewrite <- H2; auto.
+  + auto.
+  + auto.
+Qed. 
 
 Lemma proof_of_alpha_equiv_which_implies_wit_3 : alpha_equiv_which_implies_wit_3.
-Proof. Admitted. 
+Proof.
+  pre_process. 
+  sep_apply store_term'_Const; unfold NULL.
+  Intros ty1 c1.
+  sep_apply store_term'_Const; unfold NULL.
+  Intros ty2 c2.
+  Exists ty2 c2 ty1 c1.
+  entailer!.
+  + auto.
+  + rewrite <- H2; auto.
+  + auto.
+  + auto.
+Qed.
 
 Lemma proof_of_alpha_equiv_which_implies_wit_4 : alpha_equiv_which_implies_wit_4.
-Proof. Admitted. 
+Proof.
+  pre_process.
+  sep_apply store_term'_Apply; unfold NULL.
+  Intros ltt1 rtt1 yy1 zz1.
+  sep_apply store_term'_Apply; unfold NULL.
+  Intros ltt2 rtt2 yy2 zz2.
+  Exists zz2 zz1 yy2 yy1.
+  Exists ltt2 rtt2 ltt1 rtt1.
+  entailer!.
+  + auto.
+  + rewrite <- H2; auto.
+  + auto.
+  + auto.
+Qed.
 
 Lemma proof_of_alpha_equiv_which_implies_wit_5 : alpha_equiv_which_implies_wit_5.
-Proof. Admitted. 
+Proof. 
+  pre_process.
+  sep_apply store_term'_Quant; unfold NULL.
+  Intros qtt1 qvv1 bb1 yy1 zz1.
+  sep_apply store_term'_Quant; unfold NULL.
+  Intros qtt2 qvv2 bb2 yy2 zz2.
+  Exists zz2 zz1 yy2 yy1.
+  Exists qtt2 qvv2 bb2.
+  Exists qtt1 qvv1 bb1.
+  entailer!.
+  + auto.
+  + rewrite <- H2; auto.
+  + auto.
+  + auto.
+Qed.
 
 Lemma proof_of_alpha_equiv_which_implies_wit_6 : alpha_equiv_which_implies_wit_6.
-Proof. Admitted. 
+Proof.
+  pre_process.
+  rewrite H1, H2.
+  unfold store_term; fold store_term.
+  Exists y1 z1 y2 z2.
+  entailer!.
+Qed.
 
 Lemma proof_of_alpha_equiv_which_implies_wit_7 : alpha_equiv_which_implies_wit_7.
-Proof. Admitted. 
+Proof.
+  pre_process.
+  rewrite H in H0.
+  unfold termtypeID in H, H0.
+  destruct term1; try discriminate.
+  destruct term2; try discriminate.
+  unfold store_term; fold store_term.
+  Intros yy1 zz1 yy2 zz2.
+  Exists zz2 zz1 yy2 yy1.
+  Exists qtype0 qvar0 term2.
+  Exists qtype qvar term1.
+  entailer!.
+Qed. 
 
